src/SemGen.v
@@ -1,0 +1,33 @@
+Require Import ZArith List ssreflect ssrbool ssrnat.
+Require Import Axioms RoseTrees Random AbstractGen Gen.
+Import ListNotations.
+
+Set Implicit Arguments.
+
+(* Set of outcomes semantics for generators *)
+Require Import Ensembles.
+
+Definition unGen {A : Type} (g : Gen A) : RandomGen -> nat -> A :=
+  match g with MkGen f => f end.
+
+Definition semGen {A : Type} (g : Gen A) : Ensemble A :=
+  fun a => exists seed, exists size, (unGen g) seed size = a.
+
+(* Equivalence on sets of outcomes *)
+Definition set_eq {A} (m1 m2 : Ensemble A) :=
+  forall A, m1 A <-> m2 A.
+
+Infix "<-->" := set_eq (at level 70, no associativity) : pred_scope.
+
+Open Scope pred_scope.
+
+Axiom randomSeedInhabitant : RandomGen.
+
+Lemma semReturn : forall {A} (x : A),
+  semGen (returnG x) <--> eq x.
+Proof.
+  move => A x. rewrite /semGen /set_eq => a. split.
+  - move => [seed [size H]] //.
+  - move => H /=. rewrite H.
+    exists randomSeedInhabitant. exists 0. reflexivity.
+Qed.
